\documentclass{article}
\usepackage[margin = 1in]{geometry}
\usepackage{amsmath}
\begin{document}

\[
	J_P^{(l_i)} = [j_{P1}^{(l_i)} \cdots j_{Pi}^{(l_i)} 0 \cdots 0]
\]
\[ 
	j_{Pj}^{(l_i)} = z_{j-1} \times (p_{l_i} - p_{j-1}) 
\]
\[
	J_O^{(l_i)} = [j_{O1}^{(l_i)} \cdots j_{Oi}^{(l_i)} 0 \cdots 0]
\]
\[ 
	j_{Oj}^{(l_i)} = z_{j-1} 
\]

Where \( p_{j-1} \) is position vector of the origin of frame \(j-1\) and \(z_{j-1}\) is the unit vector of axis z of Frame \(j-1\), I assume written in the base frame.

\[
	J_P^{(m_i)} = [j_{P1}^{(m_i)} \cdots j_{P,i-1}^{(m_i)} 0 \cdots 0]
\]
\[ 
	j_{Pj}^{(m_i)} = z_{j-1} \times (p_{m_i} - p_{j-1}) 
\]
\[
	J_O^{(m_i)} = [j_{O1}^{(m_i)} \cdots j_{Oi}^{(m_i)} 0 \cdots 0]
\]
\[ 
	j_{Oj}^{(m_i)} = z_{m_i}, j = i, = j_{Oj}^{(l_i)}, j = 1,\cdots, i-1
\]

Where \(z_{m_i}\) denotes the unit vector of rotor rotation axis with respect to base frame.

Try $i = 1$

\begin{eqnarray*}
	j_{P1}^{(l_1)} &=& z_{0} \times (p_{l_1} - p_{0}) \\
		       &=& \begin{bmatrix} 0 \\ 0 \\ 1 \end{bmatrix} \times \left( ^0_1T\begin{bmatrix} \frac{L_1}{2} \\ 0 \\ 0 \\ 1 \end{bmatrix}  - 0 \right) = \begin{bmatrix} 0 \\ 0 \\ 1 \end{bmatrix} \times \begin{bmatrix} \frac{-s_1 L_1}{2} \\ \frac{c_1 L_1}{2} \\ 0 \end{bmatrix} \\
		       &=& \begin{bmatrix} \frac{-c_1 L_1}{2} \\ \frac{-s_1 L_1}{2} \\ 0 \end{bmatrix}
\end{eqnarray*}
Therefore:
\begin{displaymath}
	J_P^{l_1} = \begin{bmatrix} \frac{-c_1 L_1}{2} & 0 & 0 \\ \frac{-s_1 L_1}{2} & 0 & 0 \\ 0 & 0 & 0  \end{bmatrix}
\end{displaymath}

\begin{eqnarray*}
	j_{O_1}^{l_1} &=& z_{j-1} \\
		      &=& \begin{bmatrix} 0 \\ 0 \\ 1 \end{bmatrix} \\
      	J_O^{l_1} &=& \begin{bmatrix}0 & 0 & 0 \\ 0 & 0 & 0 \\ 1 & 0 & 0 \end{bmatrix}
\end{eqnarray*}

For the motor

\begin{eqnarray*}
	j_{p_1}^{m_1} &=& z_0 \times \left( p_{m_1} - p_0 \right) \\
		      &=& \begin{bmatrix} 0 \\ 0 \\ 1 \end{bmatrix} \times 0 \\
		      &=& \begin{bmatrix} 0 \\ 0 \\ 0 \end{bmatrix} \\
      	J_{P}^{m_1} &=& \begin{bmatrix} 0 & 0 & 0 \\ 0 & 0 & 0 \\ 0 & 0 & 0  \end{bmatrix} \\
      	j_{O_1}^{m_1} &=& \begin{bmatrix} 0 \\ 0 \\ 1 \end{bmatrix} \\
      	J_{O}^{m_1} &=& \begin{bmatrix} 0 & 0 & 0 \\ 0 & 0 & 0 \\ 1 & 0 & 0 \end{bmatrix}
\end{eqnarray*}

For $i = 2$

For the link:
\begin{eqnarray*}
	j_{P1}^{(l_2)} &=& z_{0}\times\left(p_{l_2} - p_{0}  \right) \\
		       &=& \begin{bmatrix} 0 \\ 0 \\ 1 \end{bmatrix} \times ^0_2T \begin{bmatrix} \frac{L_2}{2} \\ 0 \\ 0 \end{bmatrix} \\
		       &=& \begin{bmatrix} 0 \\ 0 \\ 1 \end{bmatrix} \times \begin{bmatrix} \frac{-s_{12}L_2}{2}-s_1L_1 \\ \frac{c_{12}L_2}{2} + c_1L_1 \\ 0 \end{bmatrix} \\
		       &=& \begin{bmatrix} -\frac{c_{12}L_2}{2} - c_1L_1 \\ \frac{-s_{12}L_2}{2}-s_1L_1 \\ 0 \end{bmatrix} \\
	j_{P2}^{(l_2)} &=& z_{1} \times \left(p_{l_2} - p_{1} \right) \\
		       &=& \begin{bmatrix} 0 \\ 0 \\ 1 \end{bmatrix} \times \left( \begin{bmatrix} \frac{-s_{12}L_2}{2}-s_1L_1 \\ \frac{c_{12}L_2}{2} + c_1L_1 \\ 0 \end{bmatrix} - \begin{bmatrix} -L_1s_1 \\ L_1c_1 \\ 0 \end{bmatrix} \right) \\
		       &=& \begin{bmatrix} \frac{-c_{12}L_2}{2} \\ \frac{-s_{12}L_2}{2} \\ 0 \end{bmatrix} \\
	J_{P}^{(l_2)} &=& \begin{bmatrix} -\frac{c_{12}L_2}{2} - c_1L_1 & -\frac{c_{12}L_2}{2} & 0 \\ \frac{-s_{12}L_2}{2}-s_1L_1 & \frac{-s_{12}L_2}{2} & 0 \\ 0 & 0 & 0 \end{bmatrix}
\end{eqnarray*}
\begin{eqnarray*}
	J_{O}^{(l_2)} &=& \begin{bmatrix} 0 & 0 & 0 \\ 0 & 0 & 0 \\ 1 & 1 & 0 \end{bmatrix}
\end{eqnarray*}
For the motor:
\begin{eqnarray*}
	j_{P1}^{(m_2)} &=& z_0\times\left( p_{m_2} - p_0 \right) \\
		       &=& \begin{bmatrix} 0 \\ 0 \\ 1 \end{bmatrix} \times \begin{bmatrix} -L_1 s_1 \\ L_1 c_1 \\ 0 \end{bmatrix} \\
		       &=& \begin{bmatrix}-L_1c_1 \\ -L_1s_1 \\ 0 \end{bmatrix} \\
	j_{P2}^{(m_2)} &=& 0 \text{motor is at origin of frame 1, get 0} \\
	J_{P}^{(m_2)} &=& \begin{bmatrix} -L_1 c_1 & 0 & 0 \\ -L_1 s_1 & 0 & 0 \\ 0 & 0 & 0 \end{bmatrix}
\end{eqnarray*}
\begin{eqnarray*}
	J_{O}^{(m_2)} &=& \begin{bmatrix} 0 & 0 & 0 \\ 0 & 0 & 0 \\ 1 & 1 & 0 \end{bmatrix}
\end{eqnarray*}

For $i = 3$

For the link
\begin{eqnarray*}
	j_{P1}^{(l_3)} &=& z_{0} \times \left( p_{l_3} - p_0 \right) \\
		       &=& \begin{bmatrix} 0 \\ 0 \\ 1 \end{bmatrix} \times \begin{bmatrix} -s_{12}L_2 - s_1L_1 \\ c_{12}L_2 + L_1 c_1 \\ 0 \end{bmatrix} = \begin{bmatrix} -c_{12}L_2 - L_1c_1 \\ -s_{12}L_2 - s_1L_1 \\ 0 \end{bmatrix}\\
	j_{P2}^{(l_3)} &=& z_{1} \times \left( p_{l_3} - p_1 \right) \\
		       &=& \begin{bmatrix} 0 \\ 0 \\ 1 \end{bmatrix} \times \left(\begin{bmatrix} -s_{12}L_2 - s_1L_1 \\ c_{12}L_2 + L_1 c_1 \\ 0 \end{bmatrix} - \begin{bmatrix} -L_1s_1 \\ L_1c_1 \\ 0 \end{bmatrix} \right) \\
		       &=& \begin{bmatrix} 0 \\ 0 \\ 1 \end{bmatrix} \times \begin{bmatrix} -s_{12}L_2 \\ c_{12}L_2 \\ 0 \end{bmatrix} = \begin{bmatrix} -c_{12}L_2 \\ -s_{12}L_2 \\ 0 \end{bmatrix} \\
	j_{P3}^{(l_3)} &=& z_{2} \times \left( p_{l_3} - p_2 \right) \\
		       &=& \begin{bmatrix} 0 \\ 0 \\ 0 \end{bmatrix} \\
	J_P^{(l_3)} &=& \begin{bmatrix}-c_{12}L_2 - L_1c_1 & -c_{12}L_2 & 0 \\ -s_{12}L_2 - s_1L_1 & -s_{12}L_2 & 0 \\ 0 & 0 & 0 \end{bmatrix}
\end{eqnarray*}
\begin{equation*}
	J_O^{(l_3)} = \begin{bmatrix}0 & 0 & 0 \\ 0 & 0 & 0 \\ 1 & 1 & 1 \end{bmatrix}
\end{equation*}

For the motor
\begin{eqnarray*}
	J_{P}^{(m_3)} &=& \begin{bmatrix}-c_{12}L_2 - L_1c_1 & -c_{12}L_2 & 0 \\ -s_{12}L_2 - s_1L_1 & -s_{12}L_2 & 0 \\ 0 & 0 & 0 \end{bmatrix}\\
	J_O^{(m_3)} &=& \begin{bmatrix}0 & 0 & 0 \\ 0 & 0 & 0 \\ 1 & 1 & 1 \end{bmatrix}
\end{eqnarray*}

\begin{eqnarray*}
	B(q) &=& \sum\limits_{i=1}^{n}  \left( m_{l_i} J_P^{(l_i)T}J_P^{(l_i)} + J_O^{(l_i)T}R_i I^i_{l_i} R_i^T J_O^{(l_i)} + m_{m_i} J_P^{(m_i)T} J_P^{(m_i)} + J_O^{(m_i)T} R_{m_i} I_{m_i}^{m_i} R_{m_i}^T J_O^{(m_i)} \right) \\
	B_{11} &=& I_1 + I_2 + I_3 + \left(\frac{m_2}{4} + m_3 + m_{m_3} \right)L_2^2 + \left( \frac{m_1}{4} + m_2 + m_3 + m_{m_2} + m_{m_3} \right)L_1^2 + I_{m_1} + I_{m_2} + I_{m_3} \\
	& & \hspace{.5in} + L_1 L_2 \left(m_2 + 2 m_3 + 2m_{m_3} \right) \cos \theta_2 \\
	B_{12} &=& I_2 + I_3 + \left( \frac{m_2}{4} + m_3 + m_{m_3} \right)L_2^2 + I_{m_2} + I_{m_3} + \frac{1}{2}L_1 L_2 \left(m_2 + 2m_3 + 2 m_{m_3} \right)\cos\theta_2 \\
	B_{13} &=& I_3 + I_{m_3} \\
	B_{21} &=& B_{12} \\
	B_{22} &=& I_2 + I_3 + \left(\frac{m_2}{4} + m_3 + m_{m_3} \right)L_2^2 + I_{m_2} + I_{m_3} \\
	B_{23} &=& B_{31} = B_{32} = B_{33} = B_{13}
\end{eqnarray*}
\begin{displaymath}
	g = \begin{bmatrix}\frac{1}{2} g \left( L_1 \left(m_1 + 2 m_2 + m_3 + 2 m_{m_2} \right) s_1 + L_2 m_2 s_{12} \right) \\ \frac{1}{2} g L_2 m_2 s_{12} \\ 0 \end{bmatrix}
\end{displaymath}
\begin{displaymath}
	C = \begin{bmatrix} -L_1 L_2 \left(m_2 + 2m_3 + 2m_{m_3} \right)s_2 \dot{\theta_2} & -\frac{1}{2} L_1 L_2 \left(m_2 + 2m_3 + 2m_{m_3} \right) s_2 \dot{\theta_2} & 0 \\ \frac{1}{4} L_1 L_2 \left( m_2 + 2m_3 + 2m_{m_3} \right) s_2 \left(2\dot{\theta_1} - \dot{\theta_2} \right) & \frac{1}{4}L_1 L_2 \left(m_2 + 2m_3 + 2m_{m_3} \right) s_2 \dot{\theta_1} & 0 \\ 0 & 0 & 0 \end{bmatrix}
\end{displaymath}
\begin{displaymath}
	\tau = B(q)\ddot{q} + C(q,\dot{q})\dot{q} + g(q)
\end{displaymath}
\begin{eqnarray*}
	\tau_1 &=& \frac{1}{2} g \left( L_1 \left( m_1 + 2 m_2 + m_3 + 2m_{m_2} \right) s_1 + L_2 m_2 s_{12} \right) - L_1 L_2 \left(m_2 + 2m_3 + 2m_{m_3} \right) s_2 \dot{\theta_1} \dot{\theta_2} \\
	& & \hspace{.5in} - \frac{1}{2} L_1 L_2 \left( m_2 + 2m_3 + 2 m_{m_3} \right) s_2 \dot{\theta_2}^2  + \Big(I_1 + I_2 + I_3 + L_2^2 \left(\frac{m_2}{4} + m_3 + m_{m_3} \right) \\
	& & \hspace{.5in} + L_1^2\left( \frac{m_1}{4} + m_2 + m_3 + m_{m_2} + m_{m_3} \right) + I_{m_1} + I_{m_2} + I_{m_3} + L_1 L_2 \left(m_2 + 2m_3 + 2m_{m_3} \right) c_2 \Big) \ddot{\theta_1} \\
	& & \hspace{.5in} + \left(I_2 + I_3 + L_2^2\left(\frac{m_2}{4} + m_3 + m_{m_3} \right) + I_{m_2} + I_{m_3} + \frac{1}{2}\left(m_2 +2m_3 + 2m_{m_3} \right)c_2 \right)\ddot{\theta}_2 \\
	& & \hspace{.5in} + \left(I_3 + I_{m_3}\right)\ddot{\theta}_3 \\
	\tau_2 &=& \frac{1}{4}\left(2 L_1 L_2 (m_2 + 2 m_3 +  m_{m_3} \right)s_2 \dot{\theta_1}^2 \\
	& & \hspace{.5in} \left(4I_2 + 4I_3 + L_2^2\left(m_2 + 4m_3 + 4m_{m_3} \right) + 4 I_{m_2} + 4 I_{m_3} + 2L_1 L_2 \left(m_2 + 2m_3 + 2m_{m_3} \right)c_2 \right)\ddot{\theta}_1 \\
	& & \hspace{.5in} + \left(4 I_2 + 4 I_3 + L_2^2 \left(m_2 + 4 m_3 + 4 m_{m_3} \right) + 4I_{m_2} + 4I_{m_3} \right)\ddot{\theta}_2 + \left(4I_3 + 4I_{m_3}\right)\ddot{theta}_3 \\
	\tau_3 &=& \left(I_3 + I_{m_3} \right) \left(\ddot{\theta}_1 + \ddot{\theta}_2 + \ddot{\theta}_3 \right)
\end{eqnarray*}
\end{document}